Moving lemmas from Common to Heap. Moving on Heap.

lib/Heap.v
@@ -22,17 +22,27 @@ Class BagInDec A T := {
 Section Properties.
 
 Context {A B T D : Type}
-  {BI : BagIn A T} {BE : BagEmpty T} {BR : BagRead A B T} {BRO : BagReadOption A B T} {BD : BagDom T D}.
+  {BI : BagIn A T} {BE : BagEmpty T} {BB : BagBinds A B T} {BD : BagDom T D}
+  {BR : BagRead A B T} {BRO : BagReadOption A B T}.
 
 Class ReadOption_In_eq := {
     read_option_in_eq : forall a t, a \notin t -> read_option t a = None
   }.
 
 Class ReadOption_Read_eq := {
-    read_option_read_eq : forall a b t, read_option a t = Some b -> read a t = b
+    read_option_read_eq : forall a b t, read_option t a = Some b -> read t a = b
+  }.
+
+Class In_Binds_eq := {
+    in_binds_eq : forall a t, a \in t <-> exists b, binds t a b
+  }.
+
+Class ReadOption_Binds_eq := {
+    read_option_binds_eq : forall a b t, binds t a b <-> read_option t a = Some b
   }.
 
 End Properties.
+
 
 (** ** Conversions **)
 
@@ -52,16 +62,22 @@ Qed.
 
 Definition ReadOptionToIn A B T `{BagReadOption A B T} : BagIn A T := {|
     is_in a t :=
-      match read_option t a with
-      | None => False
-      | Some _ => True
+      istrue match read_option t a with
+      | None => false
+      | Some _ => true
       end
+  |}.
+
+Definition ReadOptionToInDec A B T `{BagReadOption A B T} : BagInDec A T := {|
+    bag_in := ReadOptionToIn A B T ;
+    bag_in_dec _ _ := bool_decidable _
   |}.
 
 Instance ReadOptionToIn_ReadOption_In_eq : forall A B T `{BagReadOption A B T},
   ReadOption_In_eq (BI := ReadOptionToIn A B T).
 Proof.
-  constructors. unfold notin. simpl. introv. destruct* read_option.
+  constructors. unfold notin. simpl. introv N.
+  destruct~ read_option. false* N.
 Qed.
 
 Definition ReadToReadOption A B T `{BagRead A B T} `{BagInDec A T} : BagReadOption A B T := {|
@@ -82,6 +98,21 @@ Proof.
   rewrite decide_spec in D. rew_istrue in D. false~ E.
 Qed.
 
+Definition ReadOptionToBinds A B T `{BagReadOption A B T} : BagBinds A B T := {|
+    binds t a b :=
+      read_option t a = Some b
+  |}.
+
+Instance ReadOptionToBinds_ReadOption_Binds_eq : forall A B T `{BagReadOption A B T},
+  ReadOption_Binds_eq (BB := ReadOptionToBinds A B T).
+Proof.
+  constructors*.
+Qed.
+
+(* TODO: empty + update => single *)
+
+(* TODO: class update vs read (eq and neq) *)
+
 
 (** * Instanciation of heaps **)
 
@@ -94,7 +125,7 @@ Definition K := t.
 Module Export Tree := FMapAVL.Make(X).
 
 Instance read_option_inst V : BagReadOption K V (t V) := {|
-    read_option t a := find a t
+    read_option h k := find k h
   |}.
 
 Instance read_inst V `{Inhab V} : BagRead K V (t V) :=
@@ -102,6 +133,179 @@ Instance read_inst V `{Inhab V} : BagRead K V (t V) :=
 
 Instance in_inst V : BagIn K (t V) :=
   ReadOptionToIn K V _.
+
+Instance in_dec_inst V : BagInDec K (t V) :=
+  ReadOptionToInDec K V _.
+
+Instance binds_inst V : BagBinds K V (t V) :=
+  ReadOptionToBinds K V _.
+
+Instance empty_inst V : BagEmpty (t V) := {|
+    LibContainer.empty := Tree.empty V
+  |}.
+
+Instance update_inst V : BagUpdate K V (t V) := {|
+    update h k v := add k v h
+  |}.
+
+(* Alternative name *)
+Definition write V : t V -> K -> V -> t V := update.
+
+Instance remove_inst V : BagRemove (t V) K := {|
+    LibContainer.remove h k := Tree.remove k h
+  |}.
+
+Instance fold_inst V I : BagFold I (K -> V -> I) (t V) := {|
+    LibContainer.fold m f h :=
+      Tree.fold
+        (fun k v acc => LibMonoid.monoid_oper m (f k v) acc)
+        h
+        (LibMonoid.monoid_neutral m)
+  |}.
+
+Instance card_inst V : BagCard (t V) := {|
+    card := @cardinal _
+  |}.
+
+(* TODO: single, dom, incl *)
+
+Instance in_empty_eq V : In_empty_eq (T := t V).
+Proof. constructors*. Qed.
+
+Lemma read_option_binds : forall V (h : t V) k v,
+  read_option h k = Some v ->
+  binds h k v.
+Proof. autos~. Qed.
+
+Lemma read_option_indom : forall V (h : t V) k v,
+  read_option h k = Some v ->
+  k \indom h.
+Proof. introv E. forwards B: read_option_binds E. applys~ indom_of_binds. binds_indom B. Qed.
+
+Lemma indom_read_option : forall V (h : heap K V) k,
+  indom h k ->
+  exists v, read_option h k = Some v.
+Proof.
+  introv I. forwards (v&B): @indom_binds I.
+  exists v. applys~ @binds_read_option B.
+Qed.
+
+Lemma read_option_write_same : forall V (h : heap K V) k v,
+  read_option (write h k v) k = Some v.
+Proof. introv. apply binds_read_option. applys~ @binds_write_eq. Qed.
+
+Lemma not_indom_write : forall K V (h : heap K V) k k' v',
+  k <> k' ->
+  ~ indom h k ->
+  ~ indom (write h k' v') k.
+Proof. introv D I1 I2. forwards~: @indom_write_inv I2. Qed.
+
+Lemma read_option_write : forall V (h : heap K V) k k' v,
+  k <> k' ->
+  read_option (write h k v) k' = read_option h k'.
+Proof.
+  introv D. tests I: (indom h k').
+   forwards (v'&E): indom_read_option I. rewrite E.
+    apply read_option_binds in E. apply binds_read_option.
+    applys~ @binds_write_neq E.
+   rewrite (not_indom_read_option I). forwards I': not_indom_write I.
+    introv E. apply D. symmetry. apply* E.
+    rewrite~ (not_indom_read_option I').
+Qed.
+
+(** A notion of equivalence for heaps. **)
+Definition heap_equiv K V (h1 h2 : heap K V) :=
+  forall k v, binds h1 k v <-> binds h2 k v.
+
+Lemma heap_equiv_refl : forall K V (h : heap K V),
+  heap_equiv h h.
+Proof. introv. unfolds. autos*. Qed.
+
+Lemma heap_equiv_sym : forall K V (h1 h2 : heap K V),
+  heap_equiv h1 h2 ->
+  heap_equiv h2 h1.
+Proof. introv E. unfolds heap_equiv. introv. rewrite* E. Qed.
+
+Lemma heap_equiv_trans : forall K V (h1 h2 h3 : heap K V),
+  heap_equiv h1 h2 ->
+  heap_equiv h2 h3 ->
+  heap_equiv h1 h3.
+Proof. introv E1 E2. unfolds heap_equiv. introv. rewrite* E1. Qed.
+
+Lemma heap_equiv_binds : forall K V (h1 h2 : heap K V) k v,
+  heap_equiv h1 h2 ->
+  binds h1 k v ->
+  binds h2 k v.
+Proof. introv E B. unfolds in E. rewrite* <- E. Qed.
+
+Lemma heap_equiv_indom : forall K V (h1 h2 : heap K V) k,
+  heap_equiv h1 h2 ->
+  indom h1 k ->
+  indom h2 k.
+Proof.
+  introv E I. lets (v&B): @indom_binds I.
+  forwards B': heap_equiv_binds E B. applys~ @binds_indom B'.
+Qed.
+
+Lemma heap_equiv_read : forall V `{Inhab V} (h1 h2 : heap K V) k,
+  heap_equiv h1 h2 ->
+  indom h1 k ->
+  read h1 k = read h2 k.
+Proof.
+  introv E I. forwards (v&B): @indom_binds I.
+  rewrites >> binds_read B. symmetry. apply binds_read.
+  applys~ heap_equiv_binds E B.
+Qed.
+
+Lemma heap_equiv_read_option : forall V (h1 h2 : heap K V) k,
+  heap_equiv h1 h2 ->
+  read_option h1 k = read_option h2 k.
+Proof.
+  introv E. tests I: (indom h1 k).
+  - forwards (v&B): @indom_binds I.
+    rewrites >> (@binds_read_option) B. symmetry. apply binds_read_option.
+    applys~ heap_equiv_binds E B.
+  - do 2 rewrite~ @not_indom_read_option.
+    introv I'. false I. applys~ heap_equiv_indom I'. applys~ heap_equiv_sym E.
+Qed.
+
+Lemma heap_equiv_write : forall K V (h1 h2 : heap K V) k v,
+  heap_equiv h1 h2 ->
+  heap_equiv (write h1 k v) (write h2 k v).
+Proof.
+  introv E. unfolds heap_equiv. iff B;
+    (forwards [(?&?)|(D&B')]: @binds_write_inv B;
+     [ substs; apply binds_write_eq
+     | apply~ @binds_write_neq; applys~ heap_equiv_binds B'; apply~ heap_equiv_sym ]).
+Qed.
+
+Lemma heap_equiv_write_write : forall K V (h1 h2 : heap K V) k v v',
+  heap_equiv h1 h2 ->
+  heap_equiv (write (write h1 k v') k v) (write h2 k v).
+Proof.
+  introv E. unfolds heap_equiv. iff B;
+    (forwards [(?&?)|(D&B')]: @binds_write_inv B;
+     [ substs; apply binds_write_eq
+     | repeat apply~ @binds_write_neq ]).
+  - forwards~ B'': @binds_write_neq_inv B'. applys~ heap_equiv_binds B''.
+  - applys~ heap_equiv_binds B'. apply* heap_equiv_sym.
+Qed.
+
+Lemma heap_equiv_write_swap : forall K V (h1 h2 : heap K V) k1 k2 v1 v2,
+  k1 <> k2 ->
+  heap_equiv h1 h2 ->
+  heap_equiv (write (write h1 k1 v1) k2 v2) (write (write h2 k2 v2) k1 v1).
+Proof.
+  introv D E. unfolds heap_equiv. iff B;
+    repeat (match goal with
+    | B : binds (write _ _ _) _ _ |- _ =>
+      let D' := fresh "D" in
+      let B' := fresh "B" in
+      forwards [(?&?)|(D'&B')]: @binds_write_inv (rm B)
+    | |- binds (write _ _ _) _ _ =>
+      apply~ @binds_write_eq || apply~ @binds_write_neq
+    end; substs; tryfalse~); apply~ E.
+Qed.
 
 End HeapFromOrdered.
 
@@ -156,4 +360,8 @@ Defined.
 
 End OrderedTypeFromComparable.
 
-Module Heap (X : ComparableLt) := HeapFromOrdered (OrderedTypeFromComparable (X)).
+Module Heap (X : ComparableLt).
+Module OrderedType := OrderedTypeFromComparable X.
+Module Export Heap := HeapFromOrdered OrderedType.
+Include Heap.
+End Heap.
